%! TeX root = ./main.tex
\begin{proof}[Proof]
    Since $\Omega = \Phi(I)$, let $y$ be the coordinates on $I$, $x = \Phi(y)$,
	\[
	\int_{\Phi(I)} \nabla \varphi \dd x =
	\int_I \nabla \varphi(\Phi(y)) (\dd \Phi)^{-1} J_\Phi \dd y.
	\]
	Let $A = \dd \Phi$, WLOG $J_\Phi > 0$.
	Using the index notation and Einstein summation,
	\[
	A_{kj}A^{ji} = A^{kj}A_{ji} = \delta_{ki}.
	\]
	Thus
	\[
	\partial_{y_j}\varphi A^{ji} |A| = \partial_{y_j}(\varphi A^{ji} |A|)
	- \varphi \partial_{y_j}(A^{ji} |A|)
	\]
	Since $|A| = A_{kl}A^{kl}|A|$, $A_{kl} = \pfr{\Phi_k}{y_l}$.
	\begin{align*}
	    \partial_{y_j} (A^{ji} |A|)
		&= |A|\partial_{y_j}A^{ji} + A^{ji}\partial_{y_j}|A|\\
		&= |A|\partial_{y_j} A^{ji} + A^{ji}|A| \partial_{y_j}A_{kl}A^{kl}\\
		&= |A|(\partial_{y_j} A^{ji} + \partial_{y_l}A_{kj}A^{kl})\\
		&= |A|(\partial_{y_j}A^{ji} - \partial_{y_j}A^{ji}) = 0.
	\end{align*}
	Hence by our previous work,
	\[
	\int_I \partial_{y_j}(\varphi A^{ji} |A|)\dd y
	= \int_{\partial I} \varphi A^{ji}|A| \nu_j \dd \sigma.
	\]
	Putting this together for all $i$'s,
	note that $\wt{\nu} = \frac{\nabla \Phi^{-1}_n}{|\nabla \Phi^{-1}_n|}$,

	TODO
\end{proof}
